PremiseSelection/Cloud.lean
@@ -3,66 +3,160 @@ import Lean.Server.Utils
 
 namespace Lean.PremiseSelection.Cloud
 
-register_option apiBaseUrl : String := {
+register_option premiseSelection.apiBaseUrl : String := {
   defValue := "http://52.206.70.13"
   descr := "The base URL of the premise retrieval API"
 }
 
 def getApiBaseUrl (opts : Options) : String :=
-  apiBaseUrl.get opts
+  premiseSelection.apiBaseUrl.get opts
+
+def makeRequest {α : Type _} [FromJson α] (method urlPath : String) (data? : Option Json) : CoreM α := do
+  let apiBaseUrl := getApiBaseUrl (← getOptions)
+  let apiUrl := apiBaseUrl ++ urlPath
+  let mut curlArgs := #[
+    "-X", method,
+    "--user-agent", "LeanProver (https://leanprover-community.github.io/)"
+  ]
+  if data?.isSome then
+    curlArgs := curlArgs ++ #[
+      "--header", "Content-Type: application/json",
+      -- We put data in stdin rather than command argument, because the data may be too long
+      "--data", "@-"
+    ]
+  curlArgs := curlArgs.push apiUrl
+
+  let output : IO.Process.Output ← id <| do
+    if let some data := data? then
+      let childInit ← IO.Process.spawn { cmd := "curl", args := curlArgs, stdin := .piped, stdout := .piped, stderr := .piped }
+      let (stdin, child) ← childInit.takeStdin
+      stdin.putStr data.compress
+      let exitCode ← child.wait
+      let stdout ← child.stdout.readToEnd
+      let stderr ← child.stderr.readToEnd
+      return { exitCode, stdout, stderr }
+    else
+      IO.Process.output { cmd := "curl", args := curlArgs }
+
+  if output.exitCode != 0 then
+    IO.throwServerError <|
+      s!"Could not send API request to {apiUrl}. " ++
+      s!"curl exited with code {output.exitCode}:\n{output.stderr}"
+
+  match Json.parse output.stdout >>= fromJson? with
+  | .ok (result : α) =>
+      return result
+  | .error e => IO.throwServerError <|
+      s!"Could not parse server output (error: {e})\nRaw output:\n{output.stdout}"
 
 section IndexedPremises
 
-/-! Retrieving indexed premises and modules stored on the server -/
+/-! Retrieving indexed premises and modules stored on the server, and collecting
+new premises either imported or defined locally.
+-/
 
-/-- Unfiltered list of all premises known by the server.
-This is currently not used in Lean (but the API `/indexed-premises` will always be available). -/
-def getIndexedPremises (apiBaseUrl : String) : IO NameSet := do
-  let apiUrl := apiBaseUrl ++ "/indexed-premises"
-  let curlArgs := #[
-    "-X", "GET",
-    "--user-agent", "LeanProver (https://leanprover-community.github.io/)",
-    apiUrl
-  ]
-  let out ← IO.Process.output { cmd := "curl", args := curlArgs }
+/-- The maximum number of new premises to send to the server. -/
+def getMaxUnindexedPremises : CoreM Nat := do
+  makeRequest "GET" "/max-new-premises" none
 
-  if out.exitCode != 0 then
-    IO.throwServerError <|
-      "Could not send API request to retrieve premises. " ++
-      s!"curl exited with code {out.exitCode}:\n{out.stderr}"
+/-- A cache holding indexed premises by the server. -/
+initialize indexedPremisesRef : IO.Ref (Option NameSet) ← IO.mkRef none
+/-- Unfiltered list of all premises known by the server. The result is cached in an `IO.Ref`,
+because (assuming the server is static) the result will not change. -/
+def getIndexedPremises : CoreM NameSet := do
+  -- **TODO** this general design pattern might be generalized
+  match ← indexedPremisesRef.get with
+  | some names => return names
+  | none =>
+    let names ← core
+    indexedPremisesRef.set (some names)
+    return names
+where
+  core : CoreM NameSet := do
+    let names : Array String ← makeRequest "GET" "/indexed-premises" none
+    return names.foldl (fun ns n => ns.insert n.toName) ∅
 
-  match Json.parse out.stdout >>= fromJson? with
-  | .ok (result : Array String) =>
-      let mut names := ∅
-      for name in result do
-        names := names.insert name.toName
-      return names
-  | .error e => IO.throwServerError <|
-      s!"Could not parse server output (error: {e})"
+/-- All modules known by the server. **NOTE** This is not used. -/
+def getIndexedModules : CoreM NameSet := do
+  let moduleNames : Array String ← makeRequest "GET" "/indexed-modules" none
+  return moduleNames.foldl (fun ns n => ns.insert n.toName) ∅
 
-/-- All modules known by the server. -/
-def getIndexedModules (apiBaseUrl : String) : IO NameSet := do
-  let apiUrl := apiBaseUrl ++ "/indexed-modules"
-  let curlArgs := #[
-    "-X", "GET",
-    "--user-agent", "LeanProver (https://leanprover-community.github.io/)",
-    apiUrl
-  ]
-  let out ← IO.Process.output { cmd := "curl", args := curlArgs }
+/-- A cache holding the premises imported from other modules that are not indexed by the server. -/
+initialize unindexedImportedPremisesRef : IO.Ref (Option (Array Premise)) ← IO.mkRef none
+/-- Get the imported premises not indexed by the server. The result is cached in an `IO.Ref`,
+because (assuming the server is static) the result will not change unless the file is restarted. -/
+def getUnindexedImportedPremises (chunkSize := 256) : CoreM (Array Premise) := do
+  match ← unindexedImportedPremisesRef.get with
+  | some premises => return premises
+  | none =>
+    let premises ← core chunkSize
+    unindexedImportedPremisesRef.set (some premises)
+    return premises
+where
+  core (chunkSize : Nat) : CoreM (Array Premise) := do
+    let env ← getEnv
+    let maxUnindexedPremises ← getMaxUnindexedPremises
+    let indexedPremises ← getIndexedPremises
+    let moduleNames := env.header.moduleNames
+    let moduleData := env.header.moduleData
 
-  if out.exitCode != 0 then
-    IO.throwServerError <|
-      "Could not send API request to retrieve modules. " ++
-      s!"curl exited with code {out.exitCode}:\n{out.stderr}"
+    let mut names := #[]
+    for i in [0:moduleData.size] do
+      let moduleName := moduleNames[i]!
+      if Premise.isBlackListedModule moduleName then
+        continue
+      let modData := moduleData[i]!
+      for name in modData.constNames do
+        unless indexedPremises.contains name do
+          unless Premise.isBlackListedPremise env name do
+            names := names.push name
 
-  match Json.parse out.stdout >>= fromJson? with
-  | .ok (result : Array String) =>
-      let mut moduleNames := ∅
-      for moduleName in result do
-        moduleNames := moduleNames.insert moduleName.toName
-      return moduleNames
-  | .error e => IO.throwServerError <|
-      s!"Could not parse server output (error: {e})"
+    if names.size > maxUnindexedPremises then
+      logWarning m!"Found {names.size} unindexed premises in imports, which exceeds the maximum number of new premises ({maxUnindexedPremises}). Discarding premises beyond this limit"
+      names := names.take maxUnindexedPremises
+
+    -- `useCache := false` because the `Premise`s are cached using our `unindexedImportedPremisesRef`
+    Premise.fromNames names chunkSize false
+
+/-- Get the local premises defined in the current file that are not indexed by the server.
+
+The set of premises is not cached, to allow for adding/deleting local premises (unless indexed by the server).
+Currently, the printed signature itself is cached by the `Premise.fromName` function,
+meaning that it does not support modifying local premises,
+but (**TODO**) this behavior might (or should) change in the future either by disabling this cache
+or by making an option for users to purge cache.
+-/
+def getUnindexedLocalPremises (chunkSize := 256) : CoreM (Array Premise) := do
+  let env ← getEnv
+  let indexedPremises ← getIndexedPremises
+  let mut names := #[]
+  for (name, _) in env.constants.map₂ do
+    unless indexedPremises.contains name do
+      unless Premise.isBlackListedPremise env name do
+        names := names.push name
+  Premise.fromNames names chunkSize true -- **TODO** see docstring
+
+/-- Get the local premises defined in the current file that are indexed by the server.
+
+Modifications to these premises will *not* be reflected in the retrieval results, with
+the assumption being even if modifications are made, they should be small enough
+to significantly change the semantic meaning (the name is kept after all).
+-/
+def getIndexedLocalPremises : CoreM (Array Name) := do
+  let env ← getEnv
+  let indexedPremises ← getIndexedPremises
+  let mut names := #[]
+  for (name, _) in env.constants.map₂ do
+    if indexedPremises.contains name then
+      names := names.push name
+  return names
+
+/-- Get the new premises defined in the environment, which is the union of imported premises unindexed by the server,
+and the set of local premises in this file. -/
+def getUnindexedPremises (chunkSize := 256) : CoreM (Array Premise) := do
+  let premises₁ ← getUnindexedImportedPremises chunkSize
+  let premises₂ ← getUnindexedLocalPremises chunkSize
+  return premises₁ ++ premises₂
 
 end IndexedPremises
 
@@ -80,47 +174,17 @@ scoped instance : ToMessageData Suggestion where
 
 initialize Lean.registerTraceClass `premiseSelection.debug
 
-def selectPremisesCore (apiBaseUrl : String) (state : String)
-    (importedModules : Option (Array Name)) (newPremises : Option (Array Premise))
-    (k : Nat) : IO (Array Suggestion) := do
-  let apiUrl := apiBaseUrl ++ "/retrieve"
+def selectPremisesCore (state : String)
+    (importedModules indexedLocalPremises : Array Name) (unindexedPremises : Array Premise)
+    (k : Nat) : CoreM (Array Suggestion) := do
   let data := Json.mkObj [
     ("state", .str state),
     ("imported_modules", toJson importedModules),
-    ("new_premises", toJson newPremises),
+    ("local_premises", toJson indexedLocalPremises),
+    ("new_premises", toJson unindexedPremises),
     ("k", .num (.fromNat k)),
   ]
-  let curlArgs := #[
-    "-X", "POST",
-    "--header", "Content-Type: application/json",
-    "--user-agent", "LeanProver (https://leanprover-community.github.io/)",
-    -- We put data in stdin rather than command argument, because the data may be too long
-    "--data", "@-",
-    apiUrl
-  ]
-
-  let child ← IO.Process.spawn { cmd := "curl", args := curlArgs, stdin := .piped, stdout := .piped, stderr := .piped }
-  let (stdin, child) ← child.takeStdin
-  stdin.putStr data.compress
-  let exitCode ← child.wait
-  let stdout ← child.stdout.readToEnd
-
-  if exitCode != 0 then
-    let stderr ← child.stderr.readToEnd
-    IO.throwServerError <|
-      "Could not send API request to select premises. " ++
-      s!"curl exited with code {exitCode}:\n{stderr}"
-
-  match Json.parse stdout >>= fromJson? with
-  | .ok result => return result
-  | .error e => IO.throwServerError <|
-      s!"Could not parse premise retrieval output (error: {e})\nRaw output:\n{stdout}"
-
-/-- Get new premises in the environment that are not indexed by the server -/
-def getNewPremises (chunkSize := 256) : CoreM (Array Premise) := do
-  let indexedModules ← getIndexedModules (getApiBaseUrl (← getOptions))
-  let newPremises ← Premise.getPremises indexedModules (chunkSize := chunkSize)
-  return newPremises
+  makeRequest "POST" "/retrieve" (some data)
 
 def selectPremises (goal : MVarId) (k : Nat) : MetaM (Array Suggestion) := do
   let env ← getEnv
@@ -129,11 +193,11 @@ def selectPremises (goal : MVarId) (k : Nat) : MetaM (Array Suggestion) := do
   trace[premiseSelection.debug] m!"State: {state}"
 
   let importedModules := env.allImportedModuleNames
-  let newPremises ← getNewPremises
-  let apiBaseUrl := getApiBaseUrl (← getOptions)
+  let indexedLocalPremises ← getIndexedLocalPremises
+  let unindexedPremises ← getUnindexedPremises
 
   let suggestions ← profileitM Exception "Cloud.selectPremises" (← getOptions) do
-    selectPremisesCore apiBaseUrl state importedModules newPremises k
+    selectPremisesCore state importedModules indexedLocalPremises unindexedPremises k
 
   trace[premiseSelection.debug] m!"Suggestions: {suggestions}"
   return suggestions
