PremiseSelection/Premise.lean
@@ -56,22 +56,11 @@ def getKind (cinfo : ConstantInfo) : MetaM String := do
   return kind
 
 /-- A reference holding a mapping from a user-defined premise `name` to `Premise.fromName name` (see `Premise.fromName`). -/
-initialize Premise.fromNameCacheRef : IO.Ref (NameMap Premise) ← IO.mkRef ∅
+initialize fromNameCacheRef : IO.Ref (NameMap Premise) ← IO.mkRef ∅
 
-/--
-Serialize a declaration into a `Premise` by pretty-printing the declaration docstring and signature.
-
-This function is cached by `Premise.fromNameCacheRef`, so on the second time it is
-called on the same declaration, it reads the previously stored result instead of calculates the signature again.
-(**TODO**) This is just a temporary solution so that it is reasonable to call e.g. `aesop (add unsafe (by hammer))`
-where `hammer` is called many times.
--/
-def fromName (name : Name) : CoreM Premise := do
-  if let some premise := (← Premise.fromNameCacheRef.get).find? name then
-    return premise
-
+def fromNameCore (name : Name) : CoreM Premise := do
   -- Calculate signature from declaration name
-  let premise ← MetaM.run' do
+  MetaM.run' do
     withOptions (fun o => (o.set `pp.notation false).set `pp.fullNames true) do
       let env ← getEnv
       -- IO.eprintln name
@@ -101,8 +90,25 @@ def fromName (name : Name) : CoreM Premise := do
 
       return { name, decl }
 
-  Premise.fromNameCacheRef.modify fun cache => cache.insert name premise
-  return premise
+/--
+Serialize a declaration into a `Premise` by pretty-printing the declaration docstring and signature.
+
+If `useCache := true`, this function is cached by `fromNameCacheRef`, so on the second time it is
+called on the same declaration, it reads the previously stored result instead of calculates the signature again.
+(**TODO**) This is just a temporary solution so that it is reasonable to call e.g. `aesop (add unsafe (by hammer))`
+where `hammer` is called many times.
+-/
+def fromName (name : Name) (useCache : Bool) : CoreM Premise := do
+  if !useCache then
+    let premise ← fromNameCore name
+    return premise
+  else
+    match (← fromNameCacheRef.get).find? name with
+    | some premise => return premise
+    | none =>
+      let premise ← fromNameCore name
+      fromNameCacheRef.modify fun cache => cache.insert name premise
+      return premise
 
 /--
 Applies the monadic function `f` on every element `x` in the list, left-to-right, and returns the
@@ -120,9 +126,9 @@ def _root_.List.flatMapM {m : Type u → Type v} [Monad m] {α : Type w} {β : T
   loop as []
 
 /-- This is equivalent to `names.mapM Premise.fromName`, but it processes chunks in parallel. -/
-def fromNames (names : Array Name) (chunkSize := 256) : CoreM (Array Premise) := do
+def fromNames (names : Array Name) (chunkSize : Nat) (useCache : Bool) : CoreM (Array Premise) := do
   if chunkSize == 1 then
-    let premises ← names.mapM Premise.fromName
+    let premises ← names.mapM (Premise.fromName (useCache := useCache))
     return premises
 
   else
@@ -135,7 +141,7 @@ def fromNames (names : Array Name) (chunkSize := 256) : CoreM (Array Premise) :=
     let premiseChunkTasks ← names.toList.toChunks chunkSize |>.mapM fun names =>
       IO.asTask do
         let (premises, _) ← CoreM.toIO (ctx := ctxCore) (s := sCore) do
-          names.mapM Premise.fromName
+          names.mapM (Premise.fromName (useCache := useCache))
         return premises
     let premises ← premiseChunkTasks.flatMapM fun task => do
       IO.ofExcept (← IO.wait task)
@@ -155,6 +161,9 @@ def nameBlackList : Array String := #["Lean", "Lake", "Qq"]
 /-- A premise whose `type.getForallBody.getAppFn` is a constant that has this prefix is not retrieved. -/
 def typePrefixBlackList : Array Name := #[`Lean]
 
+def isBlackListedModule (moduleName : Name) : Bool :=
+  moduleBlackList.any (fun p => moduleName.anyS (· == p))
+
 def isBlackListedPremise (env : Environment) (name : Name) : Bool := Id.run do
   if name == ``sorryAx then return true
   if name.isInternalDetail then return true
@@ -166,48 +175,48 @@ def isBlackListedPremise (env : Environment) (name : Name) : Bool := Id.run do
     if typePrefixBlackList.any (fun p => p.isPrefixOf fnName) then return true
   return false
 
-def getModules (exclude : NameSet) : CoreM (Array ModuleData) := do
-  let env ← getEnv
-  let moduleNames := env.header.moduleNames
-  let moduleData := env.header.moduleData
-  let mut modules := #[]
+-- def getModules (exclude : NameSet) : CoreM (Array ModuleData) := do
+--   let env ← getEnv
+--   let moduleNames := env.header.moduleNames
+--   let moduleData := env.header.moduleData
+--   let mut modules := #[]
 
-  -- For each index `i` of a new module
-  for i in [0:moduleData.size] do
-    let moduleName := moduleNames[i]!
-    if exclude.contains moduleName then
-      continue
-    if moduleBlackList.any (fun p => moduleName.anyS (· == p)) then
-      continue
+--   -- For each index `i` of a new module
+--   for i in [0:moduleData.size] do
+--     let moduleName := moduleNames[i]!
+--     if exclude.contains moduleName then
+--       continue
+--     if isBlackListedModule moduleName then
+--       continue
 
-    -- Add corresponding module data
-    modules := modules.push moduleData[i]!
+--     -- Add corresponding module data
+--     modules := modules.push moduleData[i]!
 
-  return modules
+--   return modules
 
-/-- Get names of new premises in the environment -/
-def getNames (excludeModules : NameSet) : CoreM (Array Name) := do
-  let env ← getEnv
-  let mut names := #[]
-  let modules ← getModules excludeModules
+-- /-- Get names of new premises in the environment -/
+-- def getNames (excludeModules : NameSet) : CoreM (Array Name) := do
+--   let env ← getEnv
+--   let mut names := #[]
+--   let modules ← getModules excludeModules
 
-  -- All filtered constants from unindexed modules
-  for moduleData in modules do
-    for name in moduleData.constNames do
-      unless isBlackListedPremise env name do
-        names := names.push name
+--   -- All filtered constants from unindexed modules
+--   for moduleData in modules do
+--     for name in moduleData.constNames do
+--       unless isBlackListedPremise env name do
+--         names := names.push name
 
-  -- All filtered constants from this module
-  -- unless indexedMods.contains env.header.mainModule do
-  for (name, _) in env.constants.map₂ do
-    unless isBlackListedPremise env name do
-      names := names.push name
-  return names
+--   -- All filtered constants from this module
+--   -- unless indexedMods.contains env.header.mainModule do
+--   for (name, _) in env.constants.map₂ do
+--     unless isBlackListedPremise env name do
+--       names := names.push name
+--   return names
 
-/-- Get new premises in the environment -/
-def getPremises (excludeModules : NameSet) (chunkSize := 256) : CoreM (Array Premise) := do
-  let names ← getNames excludeModules
-  let premises ← fromNames names (chunkSize := chunkSize)
-  return premises
+-- /-- Get new premises in the environment -/
+-- def getPremises (excludeModules : NameSet) (chunkSize := 256) : CoreM (Array Premise) := do
+--   let names ← getNames excludeModules
+--   let premises ← fromNames names (chunkSize := chunkSize)
+--   return premises
 
 end Lean.PremiseSelection.Premise
